src/func_iter_eq/main.lean
@@ -1,0 +1,250 @@
+import tactic
+import tactic.induction
+import logic.function.iterate
+
+noncomputable theory
+open_locale classical
+
+def mem_loop {α : Type} (f : α → α) (x : α) (l : list α) : Prop :=
+∀ (n : ℕ), l.nth (n % l.length) = some ((f^[n]) x)
+
+def mem_shortest_loop {α : Type} (f : α → α) (x : α) (l : list α) : Prop :=
+mem_loop f x l ∧ ∀ (l' : list α), mem_loop f x l' → l'.length ≤ l.length
+
+-- #exit
+
+lemma iter_add {α : Type} {f : α → α} {x : α} {m n : ℕ} :
+  (f^[m + n]) x = (f^[n]) ((f^[m]) x) :=
+by rw [add_comm, function.iterate_add_apply]
+
+lemma iter_add_mul_eq_of_add_eq {α : Type}
+  {f : α → α} {x : α} {n m d : ℕ}
+  (h : (f^[n + d]) x = (f^[n]) x) :
+  (f^[n + d * m]) x = (f^[n]) x :=
+begin
+  induction m with m ih,
+  { refl },
+  { rwa [nat.mul_succ, ←nat.add_assoc, nat.add_comm n, nat.add_assoc,
+    function.iterate_add_apply, h, ←iter_add] },
+end
+
+lemma iter_mul_eq_of_eq {α : Type}
+  {f : α → α} {x : α} {m d : ℕ}
+  (h : (f^[d]) x = x) :
+  (f^[d * m]) x = x :=
+begin
+  rw ←nat.zero_add (d * m),
+  apply iter_add_mul_eq_of_add_eq,
+  rwa nat.zero_add,
+end
+
+lemma list_nth_le_eq_iff {α : Type}
+  {l : list α} {n : ℕ} {x : α} {h} :
+  l.nth_le n h = x ↔ l.nth n = some x :=
+by { rw list.nth_eq_some, tauto }
+
+lemma list_some_nth_le_eq {α : Type}
+  {l : list α} {n : ℕ} {h} :
+  some (l.nth_le n h) = l.nth n :=
+by { symmetry, rw list.nth_eq_some, tauto }
+
+lemma list_nodup_iff {α : Type} {l : list α} :
+  l.nodup ↔ ∀ (i j : ℕ), i < j → j < l.length → l.nth i ≠ l.nth j :=
+begin
+  rw list.nodup_iff_nth_le_inj,
+  simp only [list_nth_le_eq_iff, list_some_nth_le_eq],
+  split; rintro h i j h₁ h₂,
+  { exact mt (h i j (h₁.trans h₂) h₂) (ne_of_lt h₁) },
+  { intro h₃,
+    by_contra h₄,
+    wlog h₅ : i < j,
+    { exact ne_iff_lt_or_gt.mp h₄ },
+    exact h i j h₅ h₂ h₃ },
+end
+
+lemma nat_sub_lt_of_lt {a b c : ℕ} (h : a < b) : a - c < b :=
+gt_of_gt_of_ge h (nat.sub_le _ _)
+
+lemma loop_length_pos {α : Type}
+  {f : α → α} {x : α} {l : list α}
+  (h : mem_loop f x l) :
+  0 < l.length :=
+begin
+  cases l,
+  { cases h 0 },
+  { dec_trivial },
+end
+
+lemma exi_list_func_of_mem_loop {α : Type}
+  {f : α → α} {x : α} {l : list α}
+  (h : mem_loop f x l) :
+  ∃ {g : option α → option α}, ∀ (i : ℕ),
+    l.nth (i % l.length) = ((g^[i]) (some x)) :=
+begin
+  let k := l.length,
+  have hk : 0 < k := loop_length_pos h,
+  let g : option α → option α,
+  { rintro (_ | x),
+    { exact none },
+    { exact some (f x) }},
+  use g,
+  rintro i,
+  induction i with i ih,
+  { exact h 0 },
+  { rw [function.iterate_succ_apply', ←ih],
+    cases h₁ : l.nth (i % k) with y,
+    { rw list.nth_eq_none_iff at h₁,
+      contrapose! h₁,
+      exact nat.mod_lt _ hk },
+    { change _ = some (f y),
+      simp_rw [list.nth_eq_some, list_nth_le_eq_iff],
+      use [nat.mod_lt _ hk],
+      rw [h, option.some.inj_eq] at h₁ ⊢,
+      rw [function.iterate_succ_apply', h₁] }},
+end
+
+lemma nat_sub_cancel' {a b : ℕ} (h : a ≤ b) : a + (b - a) = b :=
+by rw [←nat.add_sub_assoc h, add_tsub_cancel_left]
+
+lemma nat_find_spec_lt {P : ℕ → Prop}
+  (h : ∃ (n : ℕ), P n) :
+  ∀ (n : ℕ), n < nat.find h → ¬P n :=
+λ n h₁, (nat.lt_find_iff h _).mp h₁ n (le_refl _)
+
+lemma nat_exi_mul (x y : ℕ) : ∃ (a b : ℕ), x = y * a + b :=
+by { use [x / y, x % y], rw nat.div_add_mod }
+
+lemma nat_exi_mul' {x y : ℕ}
+  (h₁ : 0 < y) (h₂ : y < x) : ∃ (a b : ℕ), b < y ∧ x = y * a + b :=
+by { use [x / y, x % y, nat.mod_lt _ h₁], rw nat.div_add_mod }
+
+-- #exit
+
+lemma nat_mul_add_mod {a b c : ℕ} : (a * b + c) % b = c % b :=
+by rw [nat.add_mod, nat.mul_mod, nat.mod_self, nat.mul_zero, nat.zero_mod,
+  nat.zero_add, nat.mod_mod]
+
+lemma nat_mul_add_mod_of_lt {a b c : ℕ} (h : c < b) : (a * b + c) % b = c :=
+by rw [nat_mul_add_mod, nat.mod_eq_of_lt h]
+
+-- #exit
+
+lemma shortest_loop_nodup {α : Type}
+  {f : α → α} {x : α} {l : list α}
+  (h : mem_shortest_loop f x l) :
+  l.nodup :=
+begin
+  cases h with hh₁ hh₂,
+  let k := l.length,
+  have hk : 0 < k := loop_length_pos hh₁,
+  obtain ⟨g, hh⟩ := exi_list_func_of_mem_loop hh₁,
+  by_contra h₁,
+  rw list_nodup_iff at h₁,
+  push_neg at h₁,
+  -- rcases h₁ with ⟨i, j, hi, hj, h₁⟩,
+  let i := nat.find h₁,
+  have hi := nat.find_spec h₁,
+  change nat.find h₁ with i at hi,
+  let j := nat.find hi,
+  have hj := nat.find_spec hi,
+  change nat.find hi with j at hj,
+  rcases hj with ⟨h₂, h₃, h₄⟩,
+  change l.length with k at h₃,
+  let d := j - i,
+  have hd₁ : 0 < d := tsub_pos_of_lt h₂,
+  have hd₂ : d < k := nat_sub_lt_of_lt h₃,
+  let x' := some x,
+  have h₆ := h₂.trans h₃,
+  have h₇ := le_of_lt h₆,
+  have hi0 : i = 0,
+  sorry { by_contra hi₁,
+    have h₅ : l.nth 0 = l.nth d,
+    { calc l.nth 0 = l.nth ((i + (k - i)) % k) :
+          by rw [nat_sub_cancel' h₇, nat.mod_self]
+        ... = (g^[i + (k - i)]) x' : by rw hh
+        ... = (g^[k - i]) ((g^[i]) x') : by rw iter_add
+        ... = (g^[k - i]) (l.nth i) : by rw [←hh, nat.mod_eq_of_lt h₆]
+        ... = (g^[k - i]) (l.nth j) : by rw h₄
+        ... = (g^[k - i]) ((g^[j]) x') : by rw [←hh, nat.mod_eq_of_lt h₃]
+        ... = (g^[j + (k - i)]) x' : by rw iter_add
+        ... = l.nth ((j + (k - i)) % k) : by rw hh
+        ... = l.nth ((d + k) % k) :
+          by rw [←nat.add_sub_assoc h₇, nat.sub_add_comm (le_of_lt h₂)]
+        ... = l.nth (d % k) : by rw nat.add_mod_right
+        ... = l.nth d : by rw nat.mod_eq_of_lt hd₂ },
+    have h₈ := nat_find_spec_lt h₁ _ (nat.pos_of_ne_zero hi₁),
+    push_neg at h₈,
+    exact h₈ _ hd₁ hd₂ h₅ },
+  have hjd : j = d := by { change _ = j - i, rw hi0, refl },
+  have hx0 : l.nth 0 = x' := by { rw [←nat.zero_mod k, hh], refl },
+  have hxd : l.nth d = x' := by rw [←hx0, ←hjd, ←hi0, h₄],
+  have hmd : ∀ (m : ℕ), l.nth ((d * m) % k) = l.nth 0,
+  sorry { intro m,
+    rw [hh, hx0],
+    apply iter_mul_eq_of_eq,
+    rwa [←hh, nat.mod_eq_of_lt hd₂] },
+  let l' := l.take d,
+  have hlen : l'.length = d,
+  sorry { rw list.length_take, exact min_eq_left (le_of_lt hd₂) },
+  specialize hh₂ l' _,
+  {
+    intro m,
+    sorry
+    -- obtain ⟨a, b, hb₁, hb₂⟩ := nat_exi_mul' hd₁ hd₂,
+    -- rw hlen,
+    -- rw nat_mul_add_mod_of_lt
+  },
+  sorry
+end
+
+#exit
+
+lemma mem_loop_nodup_of_mem_loop {α : Type}
+  {f : α → α} {x : α} {l : list α}
+  (h : mem_loop f x l) :
+  ∃ (l' : list α), l'.nodup ∧ mem_loop f x l' :=
+begin
+  sorry
+end
+
+#exit
+
+lemma mem_loop_length_le_of_mem_loop {α : Type} [fintype α]
+  {f : α → α} {x : α} {l : list α} {n : ℕ}
+  (h₁ : n = fintype.card α)
+  (h₂ : mem_loop f x l) :
+  ∃ (l' : list α), l'.length ≤ n ∧ mem_loop f x l' :=
+begin
+  sorry
+end
+
+#exit
+
+lemma exi_loop_iter_card {α : Type} [fintype α]
+  {f : α → α} {x : α} {n : ℕ}
+  (h : n = fintype.card α) :
+  ∃ (m : ℕ), 0 < m ∧ m ≤ n ∧ (f^[n+m]) x = (f^[n]) x :=
+begin
+  sorry
+end
+
+#exit
+
+lemma exi_iter_eq {α : Type} [fintype α] :
+  ∃ (a b : ℕ), a < b ∧ ∀ {f : α → α}, (f^[a]) = (f^[b]) :=
+begin
+  let n := fintype.card α,
+  use [n, n + n.factorial],
+  fsplit,
+  { exact lt_add_of_pos_right _ (nat.factorial_pos _) },
+  { intro f,
+    funext x,
+    symmetry,
+    obtain ⟨m, hm₁, hm₂, h₁⟩ := @exi_loop_iter_card α _ f x n rfl,
+    obtain ⟨a, ha⟩ := nat.dvd_factorial hm₁ hm₂,
+    rw [ha, iter_add_mul_eq_of_add_eq h₁] },
+end
+
+lemma fin_exi_iter_eq {n : ℕ} :
+  ∃ (a b : ℕ), a < b ∧ ∀ {f : fin n → fin n}, (f^[a]) = (f^[b]) :=
+exi_iter_eq
